src/coq/Theory/OOMRefinementExamples.v
@@ -23,117 +23,230 @@ From ExtLib Require Import
 Import MonadNotation.
 Import DynamicTypes.
 
-Import TopLevelBigIntptr.
-Import TopLevelRefinementsBigIntptr.
-Import DenotationTheoryBigIntptr.
-Import MCFGTheoryBigIntptr.
-Import BigIntptrInfiniteMemoryTheory.
-Import D.
-
-Import Global.
-Import Local.
-Import Stack.
-
-Import MCFGTactics.
-
 Require Import Morphisms.
 Require Import Paco.paco.
 
-Import Global.
-Import ESID.
+Module Infinite.
+  Import TopLevelBigIntptr.
+  Import TopLevelRefinementsBigIntptr.
+  Import DenotationTheoryBigIntptr.
+  Import MCFGTheoryBigIntptr.
+  Import BigIntptrInfiniteMemoryTheory.
+  Import D.
 
-Definition t_alloc : itree L0 uvalue
-  := trigger (Alloca (DTYPE_I 64%N));; ret UVALUE_None.
+  Import Global.
+  Import Local.
+  Import Stack.
 
-Definition t_ret : itree L0 uvalue
-  := ret UVALUE_None.
+  Import MCFGTactics.
 
-(* Remove allocation in infinite language *)
-Lemma remove_alloc:
-  forall g l s m,
-    refine_L6 (interp_mcfg4 TT t_alloc g (l, s) m) (interp_mcfg4 TT t_ret g (l, s) m).
-Proof.
-  intros g l s m.
-  unfold refine_L6.
-  intros t' INTERP.
-  exists t'.
-  split.
-  - cbn.
-    unfold interp_mcfg4.
-    unfold model_undef.
-    epose proof interp_prop_Proper_eq.
-    unfold Proper, respectful in *.
-    unfold Basics.flip, Basics.impl in *.
-    eapply H.
-    all: eauto; try typeclasses eauto.
-    cbn.
-    go.
+  Import Global.
+  Import ESID.
 
-    rewrite interp_memory_trigger.
-    cbn.
-    go.
-    cbn.
+  Definition t_alloc : itree L0 uvalue
+    := trigger (Alloca (DTYPE_I 64%N));; ret UVALUE_None.
 
-    pose proof (allocate_succeeds (ms_memory_stack m) (DTYPE_I 64)) as ALLOC_SUC.
-    forward ALLOC_SUC. intros CONTRA; inversion CONTRA.
+  Definition t_ret : itree L0 uvalue
+    := ret UVALUE_None.
 
-    destruct m as [ms sid pr].
-    eapply ErrSID_succeeds_ErrSID_runs_to in ALLOC_SUC as ((ms' & a) & sid' & pr' & REST).
-    rewrite REST.
+  (* Remove allocation in infinite language *)
+  Lemma remove_alloc:
+    forall g l s m,
+      refine_L6 (interp_mcfg4 TT t_alloc g (l, s) m) (interp_mcfg4 TT t_ret g (l, s) m).
+  Proof.
+    intros g l s m.
+    unfold refine_L6.
+    intros t' INTERP.
+    exists t'.
+    split.
+    - cbn.
+      unfold interp_mcfg4.
+      unfold model_undef.
+      epose proof interp_prop_Proper_eq.
+      unfold Proper, respectful in *.
+      unfold Basics.flip, Basics.impl in *.
+      eapply H.
+      all: eauto; try typeclasses eauto.
+      cbn.
+      go.
 
-    go.
-    cbn.
-    go.
-    cbn.
+      rewrite interp_memory_trigger.
+      cbn.
+      go.
+      cbn.
 
-    apply eutt_Ret.
-    reflexivity.
-  - right.
-    apply OOM.eutt_refine_oom_h; try typeclasses eauto.
-    reflexivity.
-Qed.
+      pose proof (allocate_succeeds (ms_memory_stack m) (DTYPE_I 64)) as ALLOC_SUC.
+      forward ALLOC_SUC. intros CONTRA; inversion CONTRA.
 
-(* Add allocation in infinite language *)
-Lemma add_alloc :
-  forall g l s m,
-    refine_L6 (interp_mcfg4 TT t_ret g (l, s) m) (interp_mcfg4 TT t_alloc g (l, s) m).
-Proof.
-  intros g l s m.
-  unfold refine_L6.
-  intros t' INTERP.
-  exists t'.
-  split.
-  - cbn.
-    unfold interp_mcfg4.
-    unfold model_undef.
-    epose proof interp_prop_Proper_eq.
-    unfold Proper, respectful in *.
-    unfold Basics.flip, Basics.impl in *.
-    eapply H.
-    all: eauto.
-    cbn.
-    go.
+      destruct m as [ms sid pr].
+      eapply ErrSID_succeeds_ErrSID_runs_to in ALLOC_SUC as ((ms' & a) & sid' & pr' & REST).
+      rewrite REST.
 
-    rewrite interp_memory_trigger.
-    cbn.
-    go.
-    cbn.
+      go.
+      cbn.
+      go.
+      cbn.
 
-    pose proof (allocate_succeeds (ms_memory_stack m) (DTYPE_I 64)) as ALLOC_SUC.
-    forward ALLOC_SUC. intros CONTRA; inversion CONTRA.
+      apply eutt_Ret.
+      reflexivity.
+    - right.
+      apply OOM.eutt_refine_oom_h; try typeclasses eauto.
+      reflexivity.
+  Qed.
 
-    destruct m as [ms sid pr].
-    eapply ErrSID_succeeds_ErrSID_runs_to in ALLOC_SUC as ((ms' & a) & sid' & pr' & REST).
-    rewrite REST.
+  (* Add allocation in infinite language *)
+  Lemma add_alloc :
+    forall g l s m,
+      refine_L6 (interp_mcfg4 TT t_ret g (l, s) m) (interp_mcfg4 TT t_alloc g (l, s) m).
+  Proof.
+    intros g l s m.
+    unfold refine_L6.
+    intros t' INTERP.
+    exists t'.
+    split.
+    - cbn.
+      unfold interp_mcfg4.
+      unfold model_undef.
+      epose proof interp_prop_Proper_eq.
+      unfold Proper, respectful in *.
+      unfold Basics.flip, Basics.impl in *.
+      eapply H.
+      all: eauto.
+      cbn.
+      go.
 
-    go.
-    cbn.
-    go.
-    cbn.
+      rewrite interp_memory_trigger.
+      cbn.
+      go.
+      cbn.
 
-    apply eutt_Ret.
-    reflexivity.
-  - right.
-    apply OOM.eutt_refine_oom_h; try typeclasses eauto.
-    reflexivity.
-Qed.
+      pose proof (allocate_succeeds (ms_memory_stack m) (DTYPE_I 64)) as ALLOC_SUC.
+      forward ALLOC_SUC. intros CONTRA; inversion CONTRA.
+
+      destruct m as [ms sid pr].
+      eapply ErrSID_succeeds_ErrSID_runs_to in ALLOC_SUC as ((ms' & a) & sid' & pr' & REST).
+      rewrite REST.
+
+      go.
+      cbn.
+      go.
+      cbn.
+
+      apply eutt_Ret.
+      reflexivity.
+    - right.
+      apply OOM.eutt_refine_oom_h; try typeclasses eauto.
+      reflexivity.
+  Qed.
+End Infinite.
+
+Module Finite.
+  Import TopLevel64BitIntptr.
+  Import TopLevelRefinements64BitIntptr.
+  Import DenotationTheory64BitIntptr.
+  Import MCFGTheory64BitIntptr.
+  Import D.
+
+  Import Global.
+  Import Local.
+  Import Stack.
+
+  Import MCFGTactics.
+
+  Import Global.
+  Import ESID.
+
+  Definition t_alloc : itree L0 uvalue
+    := trigger (Alloca (DTYPE_I 64%N));; ret UVALUE_None.
+
+  Definition t_ret : itree L0 uvalue
+    := ret UVALUE_None.
+
+  (* Add allocation in finite language *)
+  Lemma add_alloc :
+    forall g l s m,
+      refine_L6 (interp_mcfg4 TT t_ret g (l, s) m) (interp_mcfg4 TT t_alloc g (l, s) m).
+  Proof.
+    intros g l s m.
+    unfold refine_L6.
+    intros t' INTERP.
+    Require Import String.
+    exists (SemNotations.Ret3 g (l, s) m UVALUE_None).
+    split.
+    - cbn.
+      unfold interp_mcfg4.
+      unfold model_undef.
+      go.
+
+      epose proof interp_prop_refl.
+      unfold Proper, respectful in *.
+
+      eapply interp_prop_ret_pure; typeclasses eauto.
+    -
+      
+      right.
+      Import OOM.
+
+      unfold refine_OOM_h.
+      cbn in INTERP.
+      unfold interp_mcfg4 in INTERP.
+
+
+      Require Import Stack.
+      Require Import Global.
+      cbn.
+    Ltac go_in H :=
+      repeat match goal with
+             | H: context [interp_intrinsics (ITree.bind _ _)] |- _ => rewrite interp_intrinsics_bind in H
+             | H: context [interp_global (ITree.bind _ _)] |- _ => rewrite interp_global_bind in H
+             | H: context [interp_local_stack (ITree.bind _ _)] |- _ => rewrite interp_local_stack_bind in H
+             | H: context [interp_memory (ITree.bind _ _)] |- _ => rewrite interp_memory_bind in H
+             | H: context [interp_intrinsics (trigger _)] |- _ => rewrite interp_intrinsics_trigger in H; cbn in H; rewrite ?subevent_subevent in H
+             | H: context [interp_global (trigger _)] |- _ => rewrite interp_global_trigger in H; cbn in H; rewrite ?subevent_subevent in H
+             | H: context [interp_local_stack (trigger _)] |- _ => rewrite interp_local_stack_trigger in H; cbn in H; rewrite ?subevent_subevent in H
+             | H: context [ITree.bind (ITree.bind _ _) _] |- _ => rewrite bind_bind in H
+             | H: context [interp_intrinsics (Ret _)] |- _ => rewrite interp_intrinsics_ret in H
+             | H: context [interp_global (Ret _)] |- _ => rewrite interp_global_ret in H
+             | H: context [interp_local_stack (Ret _)] |- _ => rewrite interp_local_stack_ret in H
+             | H: context [interp_memory (Ret _)] |- _ => rewrite interp_memory_ret in H
+             | H: context [ITree.bind (Ret _) _] |- _ => rewrite bind_ret_l in H
+             end.
+
+      go_in INTERP.
+
+      unfold model_undef in INTERP.
+
+      (* I basically need to show that t' is the same as t_alloc, but
+         with a different effects signature..
+
+         I.e., it either OOMs or it returns UVALUE_None
+       *)
+
+      epose proof interp_prop_Proper_eq.
+
+      destruct (runErrSID (allocate (ms_memory_stack m) (DTYPE_I 64)) (ms_sid m) (ms_prov m))
+        as [[res sid'] pr'].
+      eapply interp_prop_Proper_eq in INTERP; try typeclasses eauto.
+      2 : {
+        go.
+        rewrite interp_memory_trigger.
+        cbn.
+        go.
+        cbn.
+      }
+
+      setoid_rewrite interp_intrinsics_trigger in INTERP.
+
+
+      rewrite interp_prop _bind in INTERP.
+
+
+      
+      cbn in GOAL.
+      
+      setoid_rewrite bind_trigger in INTERP.
+      unfolf
+      apply OOM.eutt_refine_oom_h; try typeclasses eauto.
+      reflexivity.
+  Qed.
+End Finite.
