src/coq/Theory/TopLevelRefinements.v
@@ -430,3 +430,4 @@ Module Make (IS : InterpreterStack) (TOP : LLVMTopLevel IS) : TopLevelRefinement
 End Make.
 
 Module TopLevelRefinementsBigIntptr := Make InterpreterStackBigIntptr TopLevelBigIntptr.
+Module TopLevelRefinements64BitIntptr := Make InterpreterStack64BitIntptr TopLevel64BitIntptr.
