src/coq/Utils/PropT.v
@@ -443,6 +443,21 @@ Section PropMonad.
       + eapply IHeq. reflexivity. reflexivity.   punfold HS.
   Qed.
 
+    Lemma interp_prop_ret_pure :
+      forall {T E F} (RR : relation T) `{REF: Reflexive _ RR} (x : T) (h : forall X : Type, E X -> PropT F X),
+      interp_prop h _ RR (ret x) (ret x).
+    Proof.
+      intros T E F RR REF x h.
+      generalize dependent x.
+      pcofix CIH.
+      intros x.
+      pstep.
+      cbn.
+      econstructor.
+      reflexivity.
+      reflexivity.
+    Qed.
+
     Lemma interp_prop_refl_h :
       forall {T E} (RR : relation T) `{REF: Reflexive _ RR} (t1 t2 : itree E T) (h : forall X : Type, E X -> PropT E X),
       (forall {X : Type} (e : E X), h X e (trigger e)) ->
